{
  "@context": {
    "concepts": {
      "@reverse": "skos:inScheme"
    },
    "@vocab": "http://schema.org/",
    "type": "@type",
    "id": "@id",
    "oa": "https://www.openactive.org/ns#",
    "dc": "http://purl.org/dc/terms/",
    "owl": "http://www.w3.org/2002/07/owl#",
    "rdf": "http://www.w3.org/1999/02/22-rdf-syntax-ns#",
    "rdfa": "http://www.w3.org/ns/rdfa#",
    "rdfs": "http://www.w3.org/2000/01/rdf-schema#",
    "schema": "http://schema.org/",
    "skos": "http://www.w3.org/2004/02/skos/core#",
    "xsd": "http://www.w3.org/2001/XMLSchema#",
    "pending": "http://pending.schema.org/",
    "title": "dc:title",
    "license": "dc:license",
    "prefLabel": "skos:prefLabel",
    "altLabel": "skos:altLabel",
    "inScheme": "skos:inScheme",
    "broader": "skos:broader",
    "narrower": "skos:narrower",
    "notation": "skos:notation",
    "topConceptOf": "skos:topConceptOf",
    "type": "@type",
    "Schedule": "pending:Schedule",
    "repeatFrequency": "pending:repeatFrequency",
    "repeatCount": "pending:repeatCount",
    "byDay": "pending:byDay",
    "byMonth": "pending:byMonth",
    "byMonthDay": "pending:byMonthDay",
    "exceptDate": "pending:exceptDate",
    "eventSchedule": "pending:eventSchedule",
    "ActivityOpportunity": "oa:ActivityOpportunity",
    "GenderRestrictionType": "oa:GenderRestrictionType",
    "Male": "oa:Male",
    "Female": "oa:Female",
    "None": "oa:None",
    "FacilityUse": "oa:FacilityUse",
    "ChangingRooms": "oa:ChangingRooms",
    "Showers": "oa:Showers",
    "PublicToilets": "oa:PublicToilets",
    "Lockers": "oa:Lockers",
    "Towels": "oa:Towels",
    "Creche": "oa:Creche",
    "Parking": "oa:Parking",
    "BabyChanging": "oa:BabyChanging",
    "Slot": "oa:Slot",
    "IndividualFacilityUse": "oa:IndividualFacilityUse",
    "activity": {
      "@id": "oa:activity"
    },
    "category": {
      "@id": "oa:category"
    },
    "ageRange": {
      "@id": "oa:ageRange",
      "@type": "@id"
    },
    "genderRestriction": {
      "@id": "oa:genderRestriction",
      "@type": "@id"
    },
    "programme": {
      "@id": "oa:programme"
    },
    "attendeeInstructions": {
      "@id": "oa:attendeeInstructions"
    },
    "leader": {
      "@id": "oa:leader",
      "@type": "@id"
    },
    "accessibilityInformation": {
      "@id": "oa:accessibilityInformation"
    },
    "accessibilitySupport": {
      "@id": "oa:accessibilitySupport"
    },
    "isCoached": {
      "@id": "oa:isCoached"
    },
    "level": {
      "@id": "oa:level"
    },
    "meetingPoint": {
      "@id": "oa:meetingPoint"
    },
    "facilityUse": {
      "@id": "oa:facilityUse",
      "@type": "@id"
    },
    "remainingUses": {
      "@id": "oa:remainingUses"
    },
    "maximumUses": {
      "@id": "oa:maximumUses"
    },
    "individualFacilityUse": {
      "@id": "oa:individualFacilityUse"
    }
  },
  "@graph": {
    "@context": {
      "id": "@id",
      "type": "@type",
      "dc:title": {
        "@container": "@language"
      },
      "dc:description": {
        "@container": "@language"
      },
      "dc:date": {
        "@type": "xsd:date"
      },
      "rdfs:comment": {
        "@container": "@language"
      },
      "rdfs:domain": {
        "@type": "@id"
      },
      "rdfs:label": {
        "@container": "@language"
      },
      "rdfs:range": {
        "@type": "@id"
      },
      "rdfs:seeAlso": {
        "@type": "@id"
      },
      "rdfs:subClassOf": {
        "@type": "@id"
      },
      "rdfs:subPropertyOf": {
        "@type": "@id"
      },
      "owl:equivalentClass": {
        "@type": "@vocab"
      },
      "owl:equivalentProperty": {
        "@type": "@vocab"
      },
      "owl:oneOf": {
        "@container": "@list",
        "@type": "@vocab"
      },
      "owl:imports": {
        "@type": "@id"
      },
      "owl:versionInfo": {
        "@type": "@id"
      },
      "owl:inverseOf": {
        "@type": "@vocab"
      },
      "owl:unionOf": {
        "@type": "@vocab",
        "@container": "@list"
      },
      "rdfs_classes": {
        "@reverse": "rdfs:isDefinedBy",
        "@type": "@id"
      },
      "rdfs_properties": {
        "@reverse": "rdfs:isDefinedBy",
        "@type": "@id"
      },
      "rdfs_datatypes": {
        "@reverse": "rdfs:isDefinedBy",
        "@type": "@id"
      },
      "rdfs_instances": {
        "@reverse": "rdfs:isDefinedBy",
        "@type": "@id"
      },
      "concepts": {
        "@reverse": "skos:inScheme"
      }
    },
    "@id": "https://www.openactive.org/ns#",
    "@type": "owl:Ontology",
    "dc:title": {
      "en": "OpenActive Namespace Vocabulary Terms"
    },
    "dc:description": {
      "en": "This document describes the vocabulary used in the Modelling Opportunity Data specification."
    },
    "dc:date": "2018-06-29",
    "owl:versionInfo": "https://github.com/openactive/ns/commit/d399de681a87dc6057625d70700647330ff7c826",
    "rdfs_classes": [
      {
        "@id": "oa:ActivityOpportunity",
        "@type": "rdfs:Class",
        "rdfs:label": {
          "en": "ActivityOpportunity"
        },
        "rdfs:comment": {
          "en": "An opportunity to carry out an activity at a location, at a time of the participants choosing."
        },
        "rdfs:subClassOf": "http://schema.org/Thing"
      },
      {
        "@id": "oa:GenderRestrictionType",
        "@type": "rdfs:Class",
        "rdfs:label": {
          "en": "GenderRestrictionType"
        },
        "rdfs:comment": {
          "en": "Enumerated types for gender restrictions that are applied to Events"
        }
      },
      {
        "@id": "oa:Male",
        "@type": "rdfs:Class",
        "rdfs:label": {
          "en": "Male"
        },
        "rdfs:comment": {
          "en": "Enumerated value for specifying gender restrictions"
        },
        "rdfs:subClassOf": "oa:GenderRestrictionType"
      },
      {
        "@id": "oa:Female",
        "@type": "rdfs:Class",
        "rdfs:label": {
          "en": "Female"
        },
        "rdfs:comment": {
          "en": "Enumerated value for specifying gender restrictions"
        },
        "rdfs:subClassOf": "oa:GenderRestrictionType"
      },
      {
        "@id": "oa:None",
        "@type": "rdfs:Class",
        "rdfs:label": {
          "en": "None"
        },
        "rdfs:comment": {
          "en": "Enumerated value for specifying gender restrictions"
        },
        "rdfs:subClassOf": "oa:GenderRestrictionType"
      },
      {
        "@id": "oa:FacilityUse",
        "@type": "rdfs:Class",
        "rdfs:label": {
          "en": "FacilityUse"
        },
        "rdfs:comment": {
          "en": "An opportunity to use a facility"
        },
        "rdfs:subClassOf": "schema:Product"
      },
      {
        "@id": "oa:ChangingRooms",
        "@type": "rdfs:Class",
        "rdfs:label": {
          "en": "ChangingRooms"
        },
        "rdfs:comment": {
          "en": "Changing Rooms. "
        },
        "rdfs:subClassOf": "schema:LocationFeatureSpecification"
      },
      {
        "@id": "oa:Showers",
        "@type": "rdfs:Class",
        "rdfs:label": {
          "en": "Showers"
        },
        "rdfs:comment": {
          "en": "Showers"
        },
        "rdfs:subClassOf": "schema:LocationFeatureSpecification"
      },
      {
        "@id": "oa:PublicToilets",
        "@type": "rdfs:Class",
        "rdfs:label": {
          "en": "PublicToilets"
        },
        "rdfs:comment": {
          "en": "Public Toilets"
        },
        "rdfs:subClassOf": "schema:LocationFeatureSpecification"
      },
      {
        "@id": "oa:Lockers",
        "@type": "rdfs:Class",
        "rdfs:label": {
          "en": "Lockers"
        },
        "rdfs:comment": {
          "en": "Lockers"
        },
        "rdfs:subClassOf": "schema:LocationFeatureSpecification"
      },
      {
        "@id": "oa:Towels",
        "@type": "rdfs:Class",
        "rdfs:label": {
          "en": "Towels"
        },
        "rdfs:comment": {
          "en": "Towels"
        },
        "rdfs:subClassOf": "schema:LocationFeatureSpecification"
      },
      {
        "@id": "oa:Creche",
        "@type": "rdfs:Class",
        "rdfs:label": {
          "en": "Creche"
        },
        "rdfs:comment": {
          "en": "Creche"
        },
        "rdfs:subClassOf": "schema:LocationFeatureSpecification"
      },
      {
        "@id": "oa:Parking",
        "@type": "rdfs:Class",
        "rdfs:label": {
          "en": "Parking"
        },
        "rdfs:comment": {
          "en": "Parking"
        },
        "rdfs:subClassOf": "schema:LocationFeatureSpecification"
      },
      {
        "@id": "oa:BabyChanging",
        "@type": "rdfs:Class",
        "rdfs:label": {
          "en": "BabyChanging"
        },
        "rdfs:comment": {
          "en": "BabyChanging"
        },
        "rdfs:subClassOf": "schema:LocationFeatureSpecification"
      },
      {
        "@id": "oa:Slot",
        "@type": "rdfs:Class",
        "rdfs:label": {
          "en": "Slot"
        },
        "rdfs:comment": {
          "en": "A Slot is an opportunity to use a facility at a specific time and for a specified duration. A Slot is therefore a specific type of Event, although it has a more constrained set of properties."
        },
        "rdfs:subClassOf": "schema:Event"
      },
      {
        "@id": "oa:IndividualFacilityUse",
        "@type": "rdfs:Class",
        "rdfs:label": {
          "en": "FacilityUse"
        },
        "rdfs:comment": {
          "en": "An opportunity to use a specific facility"
        },
        "rdfs:subClassOf": "oa:FacilityUse"
      }
    ],
    "rdfs_properties": [
      {
        "@id": "oa:activity",
        "@type": "rdf:Property",
        "rdfs:label": {
          "en": "activity"
        },
        "rdfs:comment": {
          "en": "Specifies the physical activity or activities that will take place during an event"
        },
        "rdfs:domain": "http://schema.org/Thing"
      },
      {
        "@id": "oa:category",
        "@type": "rdf:Property",
        "rdfs:label": {
          "en": "category"
        },
        "rdfs:comment": {
          "en": "Associate one or more tags to an Event to further categorise and describe it event, e.g. its intensity, purpose, setting, membership requirements, etc."
        },
        "rdfs:domain": "http://schema.org/Event"
      },
      {
        "@id": "oa:ageRange",
        "@type": "rdf:Property",
        "rdfs:label": {
          "en": "ageRange"
        },
        "rdfs:comment": {
          "en": "Indicates that an event is suitable for a specified age range, or that an Offer applies only to people of a specific age"
        },
        "rdfs:domain": "http://schema.org/Thing",
        "rdfs:range": "http://schema.org/QuantitativeValue"
      },
      {
        "@id": "oa:genderRestriction",
        "@type": "rdf:Property",
        "rdfs:label": {
          "en": "genderRestriction"
        },
        "rdfs:comment": {
          "en": "Indicates that an event is restricted to male, female or a mixed audience. Values should be one of the gender types specified in this vocabulary. If a gender restriction isn't specified then applications should assume that an event is suitable for a mixed audience"
        },
        "rdfs:domain": "http://schema.org/Event",
        "rdfs:range": "oa:GenderRestrictionType"
      },
      {
        "@id": "oa:programme",
        "@type": "rdf:Property",
        "rdfs:label": {
          "en": "programme"
        },
        "rdfs:comment": {
          "en": "Indicates that an event will be organised according to a specific Programme"
        },
        "rdfs:domain": "http://schema.org/Event"
      },
      {
        "@id": "oa:attendeeInstructions",
        "@type": "rdf:Property",
        "rdfs:label": {
          "en": ""
        },
        "rdfs:comment": {
          "en": "Provides additional notes and instructions for event attendees. This information is targetted at attendees rather than potential participants. The instructions might include information on what to bring, what to wear, how to find the event, etc."
        },
        "rdfs:domain": "http://schema.org/Event"
      },
      {
        "@id": "oa:leader",
        "@type": "rdf:Property",
        "rdfs:label": {
          "en": ""
        },
        "rdfs:comment": {
          "en": "The person who will be leading an event. E.g. a coach. This is a more specific role than an organiser or a contributor"
        },
        "rdfs:domain": "http://schema.org/Event",
        "rdfs:range": "http://schema.org/Person"
      },
      {
        "@id": "oa:accessibilityInformation",
        "@type": "rdf:Property",
        "rdfs:label": {
          "en": ""
        },
        "rdfs:comment": {
          "en": "Intended to capture further notes for attendees about support for disabilities or other conditions at the event"
        },
        "rdfs:domain": "http://schema.org/Event"
      },
      {
        "@id": "oa:accessibilitySupport",
        "@type": "rdf:Property",
        "rdfs:label": {
          "en": ""
        },
        "rdfs:comment": {
          "en": "What types of disabilities or conditions are accommodated at the event"
        },
        "rdfs:domain": "http://schema.org/Event"
      },
      {
        "@id": "oa:isCoached",
        "@type": "rdf:Property",
        "rdfs:label": {
          "en": ""
        },
        "rdfs:comment": {
          "en": "A boolean property that indicates whether an Event will be coached. This flag allows an Event to be marked as being coached without having to specify a named individual as a coach. This addresses both privacy concerns and also scenarios where the actual coach may only be decided on the day. "
        },
        "rdfs:domain": "http://schema.org/Event"
      },
      {
        "@id": "oa:level",
        "@type": "rdf:Property",
        "rdfs:label": {
          "en": ""
        },
        "rdfs:comment": {
          "en": "A general purpose property for specifying the suitability of an event for different participant levels. E.g. beginner/intermediate/advanced. Or in the case of martial arts, specific belt requirements. Values should ideally draw from a controlled vocabulary "
        },
        "rdfs:subPropertyOf": "http://openactive.org/ns#category",
        "rdfs:domain": "http://schema.org/Event"
      },
      {
        "@id": "oa:meetingPoint",
        "@type": "rdf:Property",
        "rdfs:label": {
          "en": ""
        },
        "rdfs:comment": {
          "en": "Instructions for the attendees of an Event about where they should meet the organizer or leader at the start of the event. Some larger locations may have several possible meeting points, so this property provides additional more specific directions."
        },
        "rdfs:subPropertyOf": "http://openactive.org/ns#attendeeInstructions",
        "rdfs:domain": "http://schema.org/Event"
      },
      {
        "@id": "oa:facilityUse",
        "@type": "rdf:Property",
        "rdfs:label": {
          "en": "facilityUse"
        },
        "rdfs:comment": {
          "en": "Associates a Slot with a FacilityUse"
        },
        "rdfs:domain": "oa:Slot",
        "rdfs:range": "oa:FacilityUse"
      },
      {
        "@id": "oa:remainingUses",
        "@type": "rdf:Property",
        "rdfs:label": {
          "en": ""
        },
        "rdfs:comment": {
          "en": "Remaining opportunities to use a Slot"
        },
        "rdfs:domain": "oa:Slot"
      },
      {
        "@id": "oa:maximumUses",
        "@type": "rdf:Property",
        "rdfs:label": {
          "en": ""
        },
        "rdfs:comment": {
          "en": "Maximum opportunities to use a Slot"
        },
        "rdfs:domain": "oa:Slot"
      },
      {
        "@id": "oa:individualFacilityUse",
        "@type": "rdf:Property",
        "rdfs:label": {
          "en": ""
        },
        "rdfs:comment": {
          "en": "Provides a list of more specific opportunities to use facilities at a location, e.g. opportunities for individual courts or pitches"
        },
        "rdfs:domain": "oa:FacilityUse"
      }
    ]
  }
}
