@prefix oa: <https://www.openactive.org/ns#> .
@prefix dc: <http://purl.org/dc/terms/> .
@prefix owl: <http://www.w3.org/2002/07/owl#> .
@prefix rdf: <http://www.w3.org/1999/02/22-rdf-syntax-ns#> .
@prefix rdfa: <http://www.w3.org/ns/rdfa#> .
@prefix rdfs: <http://www.w3.org/2000/01/rdf-schema#> .
@prefix schema: <http://schema.org/> .
@prefix skos: <http://www.w3.org/2004/02/skos/core#> .
@prefix xsd: <http://www.w3.org/2001/XMLSchema#> .
@prefix pending: <http://pending.schema.org/> .

# OpenActive Ontology definition
oa: a owl:Ontology;
  dc:title "OpenActive Namespace Vocabulary Terms"@en;
  dc:description """This document describes the vocabulary used in the Modelling Opportunity Data specification."""@en;
  dc:date "2018-05-02"^^xsd:date;
  owl:versionInfo <https://github.com/openactive/ns/commit/2d887ce73b0782e07967878d2f504a08b6b106db>;
  .


# Class definitions
oa:ActivityOpportunity a rdfs:Class;
  rdfs:label "ActivityOpportunity"@en;
  rdfs:comment """An opportunity to carry out an activity at a location, at a time of the participants choosing."""@en;
  rdfs:subClassOf http://schema.org/Thing;
  rdfs:isDefinedBy oa: .
oa:GenderRestrictionType a rdfs:Class;
  rdfs:label "GenderRestrictionType"@en;
  rdfs:comment """Enumerated types for gender restrictions that are applied to Events"""@en;
  rdfs:isDefinedBy oa: .
oa:Male a rdfs:Class;
  rdfs:label "Male"@en;
  rdfs:comment """Enumerated value for specifying gender restrictions"""@en;
  rdfs:subClassOf oa:GenderRestrictionType;
  rdfs:isDefinedBy oa: .
oa:Female a rdfs:Class;
  rdfs:label "Female"@en;
  rdfs:comment """Enumerated value for specifying gender restrictions"""@en;
  rdfs:subClassOf oa:GenderRestrictionType;
  rdfs:isDefinedBy oa: .
oa:None a rdfs:Class;
  rdfs:label "None"@en;
  rdfs:comment """Enumerated value for specifying gender restrictions"""@en;
  rdfs:subClassOf oa:GenderRestrictionType;
  rdfs:isDefinedBy oa: .
oa:FacilityUse a rdfs:Class;
  rdfs:label "FacilityUse"@en;
  rdfs:comment """An opportunity to use a facility"""@en;
  rdfs:subClassOf schema:Product;
  rdfs:isDefinedBy oa: .
oa:ChangingRooms a rdfs:Class;
  rdfs:label "ChangingRooms"@en;
  rdfs:comment """Changing Rooms. """@en;
  rdfs:subClassOf schema:LocationFeatureSpecification;
  rdfs:isDefinedBy oa: .
oa:Showers a rdfs:Class;
  rdfs:label "Showers"@en;
  rdfs:comment """Showers"""@en;
  rdfs:subClassOf schema:LocationFeatureSpecification;
  rdfs:isDefinedBy oa: .
oa:PublicToilets a rdfs:Class;
  rdfs:label "PublicToilets"@en;
  rdfs:comment """Public Toilets"""@en;
  rdfs:subClassOf schema:LocationFeatureSpecification;
  rdfs:isDefinedBy oa: .
oa:Lockers a rdfs:Class;
  rdfs:label "Lockers"@en;
  rdfs:comment """Lockers"""@en;
  rdfs:subClassOf schema:LocationFeatureSpecification;
  rdfs:isDefinedBy oa: .
oa:Towels a rdfs:Class;
  rdfs:label "Towels"@en;
  rdfs:comment """Towels"""@en;
  rdfs:subClassOf schema:LocationFeatureSpecification;
  rdfs:isDefinedBy oa: .
oa:Creche a rdfs:Class;
  rdfs:label "Creche"@en;
  rdfs:comment """Creche"""@en;
  rdfs:subClassOf schema:LocationFeatureSpecification;
  rdfs:isDefinedBy oa: .
oa:Parking a rdfs:Class;
  rdfs:label "Parking"@en;
  rdfs:comment """Parking"""@en;
  rdfs:subClassOf schema:LocationFeatureSpecification;
  rdfs:isDefinedBy oa: .
oa:BabyChanging a rdfs:Class;
  rdfs:label "BabyChanging"@en;
  rdfs:comment """BabyChanging"""@en;
  rdfs:subClassOf schema:LocationFeatureSpecification;
  rdfs:isDefinedBy oa: .
oa:Slot a rdfs:Class;
  rdfs:label "Slot"@en;
  rdfs:comment """A Slot is an opportunity to use a facility at a specific time and for a specified duration. A Slot is therefore a specific type of Event, although it has a more constrained set of properties."""@en;
  rdfs:subClassOf schema:Event;
  rdfs:isDefinedBy oa: .
oa:IndividualFacilityUse a rdfs:Class;
  rdfs:label "FacilityUse"@en;
  rdfs:comment """An opportunity to use a specific facility"""@en;
  rdfs:subClassOf oa:FacilityUse;
  rdfs:isDefinedBy oa: .

# Property definitions
oa:activity a rdf:Property;
  rdfs:label "activity"@en;
  rdfs:comment """Specifies the physical activity or activities that will take place during an event"""@en;
  rdfs:domain http://schema.org/Thing;
  rdfs:isDefinedBy oa: .
oa:category a rdf:Property;
  rdfs:label "category"@en;
  rdfs:comment """Associate one or more tags to an Event to further categorise and describe it event, e.g. its intensity, purpose, setting, membership requirements, etc."""@en;
  rdfs:domain http://schema.org/Event;
  rdfs:isDefinedBy oa: .
oa:ageRange a rdf:Property;
  rdfs:label "ageRange"@en;
  rdfs:comment """Indicates that an event is suitable for a specified age range, or that an Offer applies only to people of a specific age"""@en;
  rdfs:domain http://schema.org/Thing;
  rdfs:range http://schema.org/QuantitativeValue;
  rdfs:isDefinedBy oa: .
oa:genderRestriction a rdf:Property;
  rdfs:label "genderRestriction"@en;
  rdfs:comment """Indicates that an event is restricted to male, female or a mixed audience. Values should be one of the gender types specified in this vocabulary. If a gender restriction isn't specified then applications should assume that an event is suitable for a mixed audience"""@en;
  rdfs:domain http://schema.org/Event;
  rdfs:range oa:GenderRestrictionType;
  rdfs:isDefinedBy oa: .
oa:programme a rdf:Property;
  rdfs:label "programme"@en;
  rdfs:comment """Indicates that an event will be organised according to a specific Programme"""@en;
  rdfs:domain http://schema.org/Event;
  rdfs:isDefinedBy oa: .
oa:attendeeInstructions a rdf:Property;
  rdfs:label ""@en;
  rdfs:comment """Provides additional notes and instructions for event attendees. This information is targetted at attendees rather than potential participants. The instructions might include information on what to bring, what to wear, how to find the event, etc."""@en;
  rdfs:domain http://schema.org/Event;
  rdfs:isDefinedBy oa: .
oa:leader a rdf:Property;
  rdfs:label ""@en;
  rdfs:comment """The person who will be leading an event. E.g. a coach. This is a more specific role than an organiser or a contributor"""@en;
  rdfs:domain http://schema.org/Event;
  rdfs:range http://schema.org/Person;
  rdfs:isDefinedBy oa: .
oa:accessibilityInformation a rdf:Property;
  rdfs:label ""@en;
  rdfs:comment """Intended to capture further notes for attendees about support for disabilities or other conditions at the event"""@en;
  rdfs:domain http://schema.org/Event;
  rdfs:isDefinedBy oa: .
oa:accessibilitySupport a rdf:Property;
  rdfs:label ""@en;
  rdfs:comment """What types of disabilities or conditions are accommodated at the event"""@en;
  rdfs:domain http://schema.org/Event;
  rdfs:isDefinedBy oa: .
oa:isCoached a rdf:Property;
  rdfs:label ""@en;
  rdfs:comment """A boolean property that indicates whether an Event will be coached. This flag allows an Event to be marked as being coached without having to specify a named individual as a coach. This addresses both privacy concerns and also scenarios where the actual coach may only be decided on the day. """@en;
  rdfs:domain http://schema.org/Event;
  rdfs:isDefinedBy oa: .
oa:level a rdf:Property;
  rdfs:label ""@en;
  rdfs:comment """A general purpose property for specifying the suitability of an event for different participant levels. E.g. beginner/intermediate/advanced. Or in the case of martial arts, specific belt requirements. Values should ideally draw from a controlled vocabulary """@en;
  rdfs:subPropertyOf http://openactive.org/ns#category;
  rdfs:domain http://schema.org/Event;
  rdfs:isDefinedBy oa: .
oa:meetingPoint a rdf:Property;
  rdfs:label ""@en;
  rdfs:comment """Instructions for the attendees of an Event about where they should meet the organizer or leader at the start of the event. Some larger locations may have several possible meeting points, so this property provides additional more specific directions."""@en;
  rdfs:subPropertyOf http://openactive.org/ns#attendeeInstructions;
  rdfs:domain http://schema.org/Event;
  rdfs:isDefinedBy oa: .
oa:facilityUse a rdf:Property;
  rdfs:label "facilityUse"@en;
  rdfs:comment """Associates a Slot with a FacilityUse"""@en;
  rdfs:domain oa:Slot;
  rdfs:range oa:FacilityUse;
  rdfs:isDefinedBy oa: .
oa:remainingUses a rdf:Property;
  rdfs:label ""@en;
  rdfs:comment """Remaining opportunities to use a Slot"""@en;
  rdfs:domain oa:Slot;
  rdfs:isDefinedBy oa: .
oa:maximumUses a rdf:Property;
  rdfs:label ""@en;
  rdfs:comment """Maximum opportunities to use a Slot"""@en;
  rdfs:domain oa:Slot;
  rdfs:isDefinedBy oa: .
oa:individualFacilityUse a rdf:Property;
  rdfs:label ""@en;
  rdfs:comment """Provides a list of more specific opportunities to use facilities at a location, e.g. opportunities for individual courts or pitches"""@en;
  rdfs:domain oa:FacilityUse;
  rdfs:isDefinedBy oa: .

# Datatype definitions

# Instance definitions
